acyclic subgraph

project/sortare.dfy
@@ -73,10 +73,16 @@ method getAllIncidenceDegrees<T>(G: Graph<T>) returns (degreeMap: map<T, int>)
   }
 }
 
+predicate hasIncomingEdges<T>(G: Graph<T>, v : T)
+  requires v in G.V
+{
+  exists u :: u in G.V && ( u ,v ) in G.E
+}
 
 
 method topsort<T>(G: Graph<T>) returns (s: seq<T>)
   requires isValid(G) && acyclic(G)
+  
 {
   s := [];
   var remaining_G := G;
@@ -86,25 +92,127 @@ method topsort<T>(G: Graph<T>) returns (s: seq<T>)
                                     set e | e in G.E && e.0 !in s && e.1 !in s)
     invariant multiset(s) == multiset(G.V - remaining_G.V)
     invariant forall i, j :: 0 <= i <= j < |s| ==> (s[j], s[i]) !in G.E
+    invariant forall i :: 0 <= i < | s |
+                          ==> forall v :: v in remaining_G.V ==> ( v , s [ i ] ) !in G.E
     decreases remaining_G.V
   {
 
-    var remaining_G_V := remaining_G.V;
-    var v :| v in remaining_G.V;
-    var x := getIncidenceDegree(v, remaining_G);
+    
+    lemmaAcyclicSubgraph(remaining_G, G);
+    lemmaAcyclicIncindenceDegree(remaining_G);
+    var v :| v in remaining_G.V && ! hasIncomingEdges(remaining_G, v);
 
-    while (remaining_G_V != {} && x != 0)
-      decreases remaining_G_V
-    {
-      remaining_G_V := remaining_G_V - {v};
-      var v :| v in remaining_G.V;
-      var x := getIncidenceDegree(v, remaining_G);
-
-    }
-
-    var test1 := getIncidenceDegree(v, remaining_G);
-    assert test1 == 0;
     s := s + [v];
     remaining_G := removeVertex(v, remaining_G);
   }
 }
+
+
+lemma lemmaAcyclicIncindenceDegree<T>(G: Graph<T>)
+  requires isValid(G) && G.V != {} && acyclic (G)
+  ensures exists v :: v in G.V && !hasIncomingEdges(G, v)
+
+{
+
+  if forall v :: v in G.V ==> hasIncomingEdges(G, v) {
+    var p := generatePath(G, |G.V| + 1);
+    lemmaPathAcyclic(G, p);
+    assert !acyclic(G);
+  }
+}
+
+predicate  validPath<T>(p: seq<T>, G: Graph<T>) {
+  forall i :: 0 <= i < |p| ==> p[i] in G.V && (i < |p| - 1 ==> (p[i], p[i+1]) in G.E)
+}
+
+
+lemma generatePath<T>(G: Graph<T>, n: nat) returns (p: seq<T>)
+  requires isValid(G) && G.V != {}
+  requires forall v :: v in G.V ==> hasIncomingEdges(G, v)
+  ensures |p| == n && validPath(p, G)
+{
+  p := [];
+  while |p| < n
+    invariant |p| <= n && validPath(p, G)
+  {
+    var u :| u in G.V && (p == [] || (u, p[0]) in G.E);
+    p := [u] + p;
+  }
+}
+
+lemma lemmaPathAcyclic<T>(G: Graph<T>, p: seq<T>)
+  requires isValid(G) && validPath(p, G) && |p| > |G.V|
+  ensures !acyclic(G)
+{
+  if uniqueElements(p) {
+    lemmaSeqLength(p, G.V);
+  } else {
+    var i, j :| 0 <= i < j < |p| && p[i] == p[j];
+    var p' := p[i..j+1];
+
+    lemmaComplexPath(G, p');
+  }
+}
+
+predicate uniqueElements<T(==)>(s: seq<T>) {
+  forall i, j :: 0 <= i < j < |s| ==> s[i] != s[j]
+}
+
+function elements<T>(s: seq<T>): set<T> {
+  set x | x in s
+}
+
+lemma lemmaSeqLength<T>(p: seq<T>, s: set<T>)
+  requires uniqueElements(p) && elements(p) <= s
+  ensures |p| <= |s|
+{
+  if p != [] {
+    lemmaSeqLength(p[1..], s - {p[0]});
+  }
+}
+
+
+lemma lemmaComplexPath<T>(G: Graph<T>, p: seq<T>)
+  requires G.V != {} && validPath(p, G) && |p| > 1
+  ensures existsPath(G, p[0], p[|p| - 1])
+  decreases p
+{
+  if i :| 1 <= i < |p| - 1 && p[i] == p[0] {
+    lemmaComplexPath(G, p[i..]);
+  } else if |p| > 2 {
+    lemmaComplexPath(Graph(G.V, G.E - {(p[0], p[1])}), p[1..]);
+  }
+}
+
+////////////////////////////////////////////////////
+
+lemma lemmaAcyclicSubgraph<T>(G': Graph<T>, G: Graph<T>)
+  requires isValid(G) && isValid(G') && acyclic(G) && isSubGraph(G', G)
+  ensures acyclic(G')
+{
+  if !acyclic(G') {
+    var v :| v in G'.V && existsPath(G', v, v);
+    lemmaExistsPath(G', G, v, v);
+
+    assert !acyclic(G);
+  }
+}
+
+
+predicate isSubGraph<T>(G: Graph<T>, G': Graph<T>) {
+  G.E <= G'.E && G.V <= G'.V
+}
+
+lemma lemmaExistsPath<T>(G': Graph<T>, G: Graph<T>, u: T, v: T)
+  requires isValid(G) && isValid(G') && isSubGraph(G', G) && existsPath(G', u, v)
+  ensures existsPath(G, u, v)
+  decreases G'.E
+{
+  if (u, v) !in G'.E {
+    var e :| e in G'.E && e.0 == u && existsPath(Graph(G'.V, G'.E - {e}), e.1, v);
+
+    lemmaExistsPath(Graph(G'.V, G'.E - {e}), Graph(G.V, G.E - {e}), e.1, v);
+  }
+
+}
+
